dh.v
@@ -1,0 +1,119 @@
+From stdpp Require Import base gmap.
+From mathcomp Require Import ssreflect.
+From stdpp Require Import namespaces.
+From iris.algebra Require Import agree auth csum gset gmap excl namespace_map frac.
+From iris.base_logic.lib Require Import auth.
+From iris.heap_lang Require Import notation proofmode.
+From crypto Require Import lib guarded term crypto primitives tactics.
+
+Set Implicit Arguments.
+Unset Strict Implicit.
+Unset Printing Implicit Defensive.
+
+Section DH.
+
+Context `{!cryptoG Σ, !heapG Σ}.
+Notation iProp := (iProp Σ).
+
+Implicit Types t : term.
+Variable N : namespace.
+
+Implicit Types Ψ : val → iProp.
+Implicit Types kA kB : term.
+
+Variable P : loc → iProp.
+
+Definition dh_pred t : iProp :=
+  ∃ g a, ⌜t = TExp g [TNonce a]⌝ ∧ □ P a.
+
+Definition dh_nonce a : iProp := nonce_pred a dh_pred.
+
+Fact dh_gen_key : unit. Proof. exact: tt. Qed.
+
+Definition dh_gen g : iProp :=
+  locked_with dh_gen_key (
+    ∀ ts, [∗ set] a ∈ nonces_of_term g, published a (TExp g ts))%I.
+
+Canonical dh_gen_unlockable g := [unlockable of dh_gen g].
+
+Global Instance Persistent_dh_gen g : Persistent (dh_gen g).
+Proof. rewrite unlock; apply _. Qed.
+
+Lemma dh_gen_sterm g : dh_gen g -∗ sterm g.
+Proof.
+rewrite unlock; iIntros "H"; iSpecialize ("H" $! []).
+rewrite [in sterm _]unlock.
+iApply (big_sepS_mono with "H") => ??.
+iApply published_declared_nonce.
+Qed.
+
+Lemma nonces_of_term_dh_gen g :
+  nonces_of_term g = ∅ →
+  ⊢ dh_gen g.
+Proof.
+rewrite unlock => ->.
+by iIntros (ts); rewrite big_sepS_empty.
+Qed.
+
+Lemma dh_nonce_elim0 a :
+  dh_nonce a -∗
+  pterm (TNonce a) -∗
+  ▷ False.
+Proof.
+iIntros "#aP #p_t".
+rewrite pterm_TNonce.
+iPoseProof (publishedE with "aP p_t") as "{p_t} p_t".
+iIntros "!>".
+iDestruct "p_t" as (g' a') "# [%e p_t]".
+by move/(f_equal is_exp): e; rewrite is_exp_TExp.
+Qed.
+
+Lemma dh_nonce_elim1 g a :
+  dh_nonce a -∗
+  pterm (TExp g [TNonce a]) -∗
+  ▷ P a.
+Proof.
+iIntros "#aP #p_t".
+rewrite pterm_TExp1 big_sepS_union_pers.
+iDestruct "p_t" as "[[? contra]|[_ p_t]]".
+  by iPoseProof (dh_nonce_elim0 with "aP contra") as ">[]".
+rewrite nonces_of_term_eq /= big_sepS_singleton.
+iPoseProof (publishedE with "aP p_t") as "{p_t} p_t".
+iIntros "!>".
+iDestruct "p_t" as (g' a') "# [%e p_t]".
+by case/TExp_inj: e => _ /Permutation_singleton [] ->; eauto.
+Qed.
+
+Lemma dh_nonce_elim2 g a t :
+  dh_nonce a -∗
+  pterm (TExp g [TNonce a; t]) -∗
+  ◇ (pterm (TExp g [TNonce a]) ∧ pterm t).
+Proof.
+iIntros "#aP #p_t".
+rewrite pterm_TExp2 !big_sepS_union_pers.
+iDestruct "p_t" as "[[??] | [[? contra] | p_t]]"; eauto.
+  by iPoseProof (dh_nonce_elim0 with "aP contra") as ">[]".
+iDestruct "p_t" as "([_ p_t] & _)".
+rewrite nonces_of_term_eq /= big_sepS_singleton.
+iPoseProof (publishedE with "aP p_t") as "{p_t} p_t".
+iAssert (▷ False)%I as ">[]".
+iModIntro.
+iDestruct "p_t" as (g' a') "(%e & _)".
+by case/TExp_inj: e => _ /Permutation_length.
+Qed.
+
+Lemma dh_pterm_TExp g a :
+  dh_gen g -∗
+  dh_nonce a -∗
+  ▷ □ P a -∗
+  pterm (TExp g [TNonce a]).
+Proof.
+rewrite unlock; iIntros "#gP #aP #P_a".
+rewrite pterm_TExp1; iRight.
+rewrite big_sepS_union_pers; iSplit; first by iApply "gP".
+rewrite nonces_of_term_eq /= big_sepS_singleton.
+iExists _; iSplit; eauto.
+by iExists g, a; eauto.
+Qed.
+
+End DH.
